Engine/PikeSubset.v
@@ -1,0 +1,178 @@
+Require Import List Lia.
+Import ListNotations.
+
+From Linden Require Import Regex Chars Groups.
+From Linden Require Import Tree Semantics.
+From Warblre Require Import Numeric Base.
+
+(* The subset of regexes supported by the PikeVM engine *)
+
+Context `{characterClass: Character.class}.
+
+
+(** * PikeVM supported subset  *)
+
+Inductive pike_regex : regex -> Prop :=
+| pike_eps:
+  pike_regex Epsilon
+| pike_char:
+  forall cd, pike_regex (Regex.Character cd)
+| pike_disj:
+  forall r1 r2,
+    pike_regex r1 ->
+    pike_regex r2 ->
+    pike_regex (Disjunction r1 r2)
+| pike_seq:
+  forall r1 r2,
+    pike_regex r1 ->
+    pike_regex r2 ->
+    pike_regex (Sequence r1 r2)
+| pike_star:
+  forall r1,
+    pike_regex r1 ->
+    pike_regex (Quantified true 0 NoI.Inf r1)
+| pike_group:
+  forall g r1,
+    pike_regex r1 ->
+    pike_regex (Group g r1).
+
+(* lifting to actions *)
+Inductive pike_action: action -> Prop :=
+| pike_areg:
+  forall r1,
+    pike_regex r1 ->
+    pike_action (Areg r1)
+| pike_aclose: forall g, pike_action (Aclose g)
+| pike_acheck: forall s, pike_action (Acheck s).
+
+(* lifting to actions lists *)
+Inductive pike_actions: actions -> Prop :=
+| pike_nil: pike_actions []
+| pike_cons: forall a l,
+    pike_action a ->
+    pike_actions l ->
+    pike_actions (a::l).
+
+(* only a subset of trees can correspond to a pike regex *)
+Inductive pike_subtree: tree -> Prop :=
+| pike_mismatch: pike_subtree Mismatch
+| pike_match: pike_subtree Match
+| pike_choice: forall t1 t2,
+    pike_subtree t1 -> pike_subtree t2 ->
+    pike_subtree (Choice t1 t2)
+| pike_read: forall cd t1,
+    pike_subtree t1 ->
+    pike_subtree (Read cd t1)
+| pike_progress: forall str t1,
+    pike_subtree t1 ->
+    pike_subtree (Progress str t1)
+| pike_groupaction: forall ga t1,
+    pike_subtree t1 ->
+    pike_subtree (GroupAction ga t1).
+
+(* used for the lists of trees and gm manipulated by the PikeTree algorithm *)
+Definition pike_list (l: list (tree * group_map)) : Prop :=
+  (forall t gm, In (t, gm) l -> pike_subtree t).
+
+
+(** * Subset Properties  *)
+
+Lemma pike_list_cons:
+  forall t gm l,
+    pike_list ((t,gm)::l) -> pike_subtree t /\ pike_list l.
+Proof.
+  intros t gm l H. unfold pike_list in *. split.
+  - eapply H; eauto. left. eauto.
+  - intros. eapply H; eauto. right. eauto.
+Qed.
+
+Lemma pike_list_app:
+  forall l1 l2,
+    pike_list (l1 ++ l2) <-> pike_list l1 /\ pike_list l2.
+Proof.
+  intros l1 l2. unfold pike_list. split; try split; intros.
+  - eapply H. rewrite in_app_iff. left. eauto.
+  - eapply H. rewrite in_app_iff. right. eauto.
+  - destruct H. rewrite in_app_iff in H0. destruct H0.
+    + eapply H; eauto.
+    + eapply H1; eauto.
+Qed.
+
+Lemma pike_list_empty:
+  pike_list [].
+Proof.
+  unfold pike_list. intros. inversion H.
+Qed.
+
+Lemma pike_list_single:
+  forall t gm, pike_subtree t -> pike_list [(t,gm)].
+Proof.
+  unfold pike_list. intros t gm H t0 gm0 H0. inversion H0; inversion H1; subst; auto.
+Qed.
+
+Lemma pike_list_twice:
+  forall t1 t2 gm1 gm2, pike_subtree t1 -> pike_subtree t2 -> pike_list [(t1,gm1);(t2,gm2)].
+Proof.
+  unfold pike_list. intros t1 t2 gm1 gm2 H H0 t gm H1.
+  inversion H1; inversion H2; try inversion H3; subst; auto.
+Qed.
+
+
+
+
+(* inverting evidence of belonging to the subset *)
+Ltac invert_subset := 
+  match goal with
+  | [ H : pike_list ((_,_)::_) |- _ ] => apply pike_list_cons in H; destruct H
+  | [ H : pike_list (?tgm::_) |- _ ] => destruct ?tgm
+  | [ H : pike_list (_ ++ _) |- _ ] => apply pike_list_app in H; destruct H
+    
+  | [ H : pike_subtree (Choice _ _) |- _ ] => inversion H; clear H
+  | [ H : pike_subtree (Read _ _) |- _ ] => inversion H; clear H
+  | [ H : pike_subtree (Progress _ _) |- _ ] => inversion H; clear H
+  | [ H : pike_subtree (GroupAction _ _) |- _ ] => inversion H; clear H
+  | [ H : pike_subtree (ReadBackRef _ _) |- _ ] => inversion H; clear H
+  | [ H : pike_subtree (AnchorPass _ _) |- _ ] => inversion H; clear H
+  | [ H : pike_subtree (LK _ _ _) |- _ ] => inversion H; clear H
+  | [ H : pike_subtree (LKFail _ _) |- _ ] => inversion H; clear H                                       
+
+  | [ H : pike_actions (_ :: _) |- _ ] => inversion H; clear H
+
+  | [ H : pike_action (Areg _) |- _ ] => inversion H; clear H
+                                                           
+  | [ H : pike_regex (Regex.Character _) |- _ ] => inversion H; clear H
+  | [ H : pike_regex (Disjunction _ _) |- _ ] => inversion H; clear H
+  | [ H : pike_regex (Sequence _ _) |- _ ] => inversion H; clear H
+  | [ H : pike_regex (Quantified _ _ _ _) |- _ ] => inversion H; clear H
+  | [ H : pike_regex (Group _ _) |- _ ] => inversion H; clear H
+  | [ H : pike_regex (Lookaround _ _) |- _ ] => inversion H; clear H
+  | [ H : pike_regex (Anchor _) |- _ ] => inversion H; clear H
+  | [ H : pike_regex (Backreference _) |- _ ] => inversion H; clear H
+
+  | [ |- pike_list (_ ++ _) ] => apply pike_list_app; split
+  | [ |- pike_list [] ] => apply pike_list_empty
+  | [ |- pike_list [(_,_)] ] => apply pike_list_single
+  | [ |- pike_list [(_,_);(_,_)] ] => apply pike_list_twice
+  | [ |- pike_list [?tgm] ] => destruct ?tgm
+
+  end.
+
+Ltac pike_subset :=
+  repeat (invert_subset; subst); repeat (constructor; auto).
+
+
+(* prove that one can only construct pike subtrees from pike regexes *)
+Lemma pike_actions_pike_tree:
+  forall cont inp gm dir t,
+    pike_actions cont ->
+    is_tree cont inp gm dir t ->
+    pike_subtree t.
+Proof.
+  intros cont inp gm dir t PIKE ISTREE.
+  induction ISTREE; try apply IHISTREE; pike_subset; auto.
+  - apply IHISTREE1. pike_subset. 
+  - apply IHISTREE2. pike_subset.
+  - destruct dir; simpl; pike_subset. 
+  - apply IHISTREE1. pike_subset. destruct plus; inversion H3. constructor. auto.
+  - apply IHISTREE. pike_subset.
+Qed.
